---
title:  'Programming languages - U6'
author:
- Jan Dietrich - 10-100-436
keywords: [Programming, languages]
description: |
    programming
    languages
...


# 1

Given:

$t \equiv \lambda f . \lambda n_1 . \lambda n_2 . \textrm{if }(\text{isZero } n_1)\ 0\ (\textrm{add } n_2 (f(\textrm{pred } n_1) n_2)$

and 

$(((Yt)1)k) \rightarrow k$

we can replace the insert the values for $n_1, n_2, f$

$\textrm{if }(\text{isZero } 1)\ 0\ (\textrm{add } k ((Yt)(\textrm{pred } 1) k)$

with $\textrm{isZero }1=\textrm{false}$ und $\textrm{pred }1=0$

$\textrm{add } k ((Yt)0 k$

since we have 

$Y t \leftrightarrow t( Y t)$

we can reuse the function definition to achieve

$\textrm{add } k (( \lambda f . \lambda n_1 . \lambda n_2 . \textrm{if }(\text{isZero } n_1)\ 0\ (\textrm{add } n_2 (f(\textrm{pred } n_1) n_2))0 k$

with $\textrm{isZero }n_1$ with $n_1 = 0$ is $\textrm{true}$ results in

$\textrm{add }k 0$

since we know the implementation of add we can safely say

$\textrm{add }k\ 0 =k$


# 2 

replace append with a $f$

$\textrm{app} \equiv \lambda f . \lambda l_1 . \lambda l_2 . \textrm{if }(\textrm{null }l_1) l_2 (\textrm{cons }( \textrm{head }l_1)(f(\textrm{tail }l_1)l_2))$

To test insert $L_1 = \textrm{cons }1 (\textrm{cons }2\ \textrm{nil})$ and $L_2 = \textrm{cons }3\ \textrm{nil}$

$\textrm{if }(\textrm{null }(\textrm{cons }1 (\textrm{cons }2\ \textrm{nil})) (\textrm{cons }3\ \textrm{nil}) (\textrm{cons }( \textrm{head }(\textrm{cons }1 (\textrm{cons }2\ \textrm{nil})))(f(\textrm{tail }(\textrm{cons }1 (\textrm{cons }2\ \textrm{nil})))(\textrm{cons }3\ \textrm{nil}))$

since it's pretty unreadable we try to simplify

we can simplify the head and tail parts

$\textrm{if }(\textrm{null }(\textrm{cons }1 (\textrm{cons }2\ \textrm{nil})) (\textrm{cons }3\ \textrm{nil}) (\textrm{cons }( \textrm{cons }1 )(f(\textrm{cons }2\ \textrm{nil})(\textrm{cons }3\ \textrm{nil}))$

next step we can simplify cons

$\textrm{if }(\textrm{null }(\textrm{cons }1 (\textrm{cons }2\ \textrm{nil})) (\textrm{cons }3\ \textrm{nil}) (\textrm{cons }1(f(\textrm{cons }2\ \textrm{nil})(\textrm{cons }3\ \textrm{nil}))$

we now that $\textrm{null }(\textrm{cons }1 (\textrm{cons }2\ \textrm{nil}))$ must be $\textrm{false}$

$\textrm{cons }1(f(\textrm{cons }2\ \textrm{nil})(\textrm{cons }3\ \textrm{nil}))$

and since 
$Y \textrm{app} \leftrightarrow \textrm{app}( Y \textrm{app})$

$\textrm{cons }1(\textrm{app }(Y \textrm{app })(\textrm{cons }2\ \textrm{nil})(\textrm{cons }3\ \textrm{nil}))$

By inserting the $\textrm{app}$ definition



$\textrm{cons }1(\lambda f . \lambda l_1 . \lambda l_2 . \textrm{if }(\textrm{null }l_1) l_2 (\textrm{cons }( \textrm{head }l_1)(f(\textrm{tail }l_1)l_2))(Y \textrm{app })(\textrm{cons }2\ \textrm{nil})(\textrm{cons }3\ \textrm{nil}))$

with null cons $2$ nil $= \textrm{false}$ and head (cons 2 nil) = 2 and tail cons 2 nil = nil


$\textrm{cons }1(\textrm{cons }2((Y \textrm{app })\textrm{nil }(\textrm{cons }3\ \textrm{nil})$

again use $\textrm{app}$ definition with $l_1 = \textrm{nil}$

and since we now have

$\textrm{null }\textrm{nil }$ which results to $\textrm{true}$

we can simpify to

$\textrm{cons }1(\textrm{cons }2( \textrm{cons }3\ \textrm{nil})$

In the example there is written that this is equivalent to [1,2,3] 
